src/burrow/parity.v
@@ -1,0 +1,45 @@
+From iris.prelude Require Import options.
+From stdpp Require Import numbers.
+Require Import coq_tricks.Deex.
+
+Inductive Parity :=
+| Even : nat -> Parity
+| Odd : nat -> Parity.
+
+Fixpoint parity (n: nat) : Parity :=
+  match n with
+  | 0 => Even 0
+  | S 0 => Odd 0
+  | S (S i) => match parity i with
+      | Even k => Even (k + 1)
+      | Odd k => Odd (k + 1)
+      end
+  end.
+
+Definition even_get (n: nat) : option nat :=
+    match parity n with Even k => Some k | Odd _ => None end.
+    
+Definition odd_get (n: nat) : option nat :=
+    match parity n with Odd k => Some k | Even _ => None end.
+    
+Lemma parity_2i (i: nat) : parity (2*i) = Even i.
+Proof. induction i.
+ - simpl. trivial.
+ - replace (2 * S i) with (S (S (2 * i))) by lia.
+   unfold parity in *. rewrite IHi. f_equal. lia.
+Qed.
+
+Lemma parity_2i_1 (i: nat) : parity (2*i + 1) = Odd i.
+Proof. induction i.
+ - simpl. trivial.
+ - replace (2 * S i + 1) with (S (S (2 * i + 1))) by lia.
+   unfold parity in *. rewrite IHi. f_equal. lia.
+Qed.
+
+Lemma even_or_odd (i: nat) : (∃ k , i = 2*k) \/ (∃ k , i = 2*k + 1).
+Proof. induction i.
+  - left. exists 0. lia.
+  - destruct IHi.
+    + right. deex. exists k. lia.
+    + left. deex. exists (k+1). lia.
+Qed.
